Finished all proofs in key-value store implementation!
Woohoo!  The key was to barf on deserializing unsorted lists, so that
in the cases that we do anything at all, we do the correct thing.

The implementation is one monster of a file, at 2053 lines <_<  >_>

SerializableMergableFMapImplementation.v
@@ -1390,12 +1390,165 @@ Module MakeSerializableMergableMap (E : SerializableOrderedType) (M : Sfun E) <:
       cleanup. }
   Qed.
 
+  Fixpoint is_sorted {elt} (elements : list (M.key * (nat * option elt)))
+  : bool
+    := match elements with
+         | nil => true
+         | x::xs => match xs with
+                      | nil => true
+                      | y::ys => match E.compare (fst x) (fst y) with
+                                   | LT _ => is_sorted xs
+                                   | EQ _ => false
+                                   | GT _ => false
+                                 end
+                    end
+       end.
+
+  Lemma Sorted_is_sorted {elt} ls
+  : @is_sorted elt ls = true <-> Sorted (@M.lt_key _) ls.
+  Proof.
+    rewrite Sorted_LocallySorted_iff.
+    induction ls; simpl; split; intros; try constructor; simpl in *;
+    split_iff;
+    generalize dependent (is_sorted ls); intros;
+    destruct ls; simpl in *; try constructor;
+    repeat match goal with
+             | [ H : LocallySorted _ (_::_::_) |- _ ] => (inversion H; clear H)
+             | _ => progress intuition subst
+             | _ => progress hnf in *
+             | [ H : E.lt ?a ?b |- _ ] => unique pose proof (E.lt_not_eq H : _ -> False)
+             | [ H : E.lt ?a ?b, H' : E.lt ?b ?c |- _ ] => unique pose proof (E.lt_trans H H')
+           end;
+    edestruct E.compare;
+    repeat match goal with
+             | _ => progress subst
+             | [ H : E.lt ?a ?b |- _ ] => unique pose proof (E.lt_not_eq H : _ -> False)
+             | [ H : E.lt ?a ?b, H' : E.lt ?b ?c |- _ ] => unique pose proof (E.lt_trans H H')
+             | [ H : False |- _ ] => destruct H
+             | [ H : E.eq ?a ?a -> False |- _ ] => unique pose proof (H (E.eq_refl _))
+             | _ => eauto; congruence
+           end.
+  Qed.
+
+  Lemma not_Sorted_is_sorted {elt} ls
+  : @is_sorted elt ls = false <-> ~Sorted (@M.lt_key _) ls.
+  Proof.
+    rewrite <- Sorted_is_sorted.
+    destruct (is_sorted ls); split; congruence.
+  Qed.
+
+  Local Instance eq_prod_lt_compat {A R}
+  : Proper
+      (E.eq * R ==> E.eq * R ==> iff)
+      (@M.lt_key A).
+  Proof.
+    lazy; intros; destruct_head prod; split; destruct_head and; intros;
+    match goal with
+      | [ H : E.eq ?b ?a, H' : E.lt ?b ?c, H'' : E.eq ?c ?d |- E.lt ?a ?d ]
+        => destruct (E.compare a d); trivial; destruct (E.compare a c); destruct (E.compare b d)
+      | [ H : E.eq ?a ?b, H' : E.lt ?b ?c, H'' : E.eq ?d ?c |- E.lt ?a ?d ]
+        => destruct (E.compare a d); trivial; destruct (E.compare a c); destruct (E.compare b d)
+    end;
+    repeat match goal with
+             | [ H : False |- _ ] => destruct H
+             | [ H : E.eq ?x ?y |- _ ]
+               => unique pose proof (E.eq_sym H)
+             | [ x : key |- _ ]
+               => unique pose proof (E.eq_refl x)
+             | [ H : E.eq ?x ?y, H' : E.eq ?y ?z |- _ ]
+               => unique pose proof (E.eq_trans H H')
+             | [ H : E.lt ?x ?y, H' : E.lt ?y ?z |- _ ]
+               => unique pose proof (E.lt_trans H H')
+             | [ H : E.lt ?x ?y, H' : E.eq ?x ?y |- _ ]
+               => unique pose proof (E.lt_not_eq H H')
+           end.
+  Qed.
+
+  Local Instance eq_lt_compat {A}
+  : Proper
+      (@eq_key A ==> @eq_key A ==> iff)
+      (@M.lt_key A).
+  Proof.
+    lazy; intros; destruct_head prod; split; intros;
+    match goal with
+      | [ H : E.eq ?b ?a, H' : E.lt ?b ?c, H'' : E.eq ?c ?d |- E.lt ?a ?d ]
+        => destruct (E.compare a d); trivial; destruct (E.compare a c); destruct (E.compare b d)
+      | [ H : E.eq ?a ?b, H' : E.lt ?b ?c, H'' : E.eq ?d ?c |- E.lt ?a ?d ]
+        => destruct (E.compare a d); trivial; destruct (E.compare a c); destruct (E.compare b d)
+    end;
+    repeat match goal with
+             | [ H : False |- _ ] => destruct H
+             | [ H : E.eq ?x ?y |- _ ]
+               => unique pose proof (E.eq_sym H)
+             | [ x : key |- _ ]
+               => unique pose proof (E.eq_refl x)
+             | [ H : E.eq ?x ?y, H' : E.eq ?y ?z |- _ ]
+               => unique pose proof (E.eq_trans H H')
+             | [ H : E.lt ?x ?y, H' : E.lt ?y ?z |- _ ]
+               => unique pose proof (E.lt_trans H H')
+             | [ H : E.lt ?x ?y, H' : E.eq ?x ?y |- _ ]
+               => unique pose proof (E.lt_not_eq H H')
+           end.
+  Qed.
+
+  Lemma Sorted_eqlistA {elt} {R'} `{Transitive elt R'} {R : relation elt} ls ls'
+        `{Proper _ (R ==> R ==> iff)%signature R'}
+  : eqlistA R ls ls' -> (Sorted R' ls <-> Sorted R' ls').
+  Proof.
+    rewrite !Sorted_LocallySorted_iff.
+    revert ls'; induction ls; intros ls' HE.
+    { inversion HE; subst; reflexivity. }
+    { split; intro Hls; inversion Hls; clear Hls; subst;
+      inversion HE; clear HE; subst;
+      repeat match goal with
+               | _ => progress subst
+               | _ => progress split_iff
+               | [ H : eqlistA _ _ nil |- _ ] => (inversion H; clear H)
+               | [ H : eqlistA _ nil _ |- _ ] => (inversion H; clear H)
+               | [ H : eqlistA _ (_::_) ?x |- _ ] => (atomic x; inversion H)
+               | [ H : eqlistA _ ?x (_::_) |- _ ] => (atomic x; inversion H)
+               | _ => solve [ constructor | eauto ]
+               | [ |- LocallySorted _ (_::_::_) ] => constructor; eauto
+               | _ => progress unfold Proper, respectful, impl in *
+             end. }
+  Qed.
+
+  Local Instance eq_key_Equivalence {A} : Equivalence (@eq_key A).
+  Proof.
+    split; typeclasses eauto.
+  Qed.
+
+  Local Instance lt_key_StrictOrder {A} : StrictOrder (@M.lt_key A).
+  Proof.
+    split.
+    { intros x H'.
+      apply E.lt_not_eq in H'.
+      apply H', E.eq_refl. }
+    { intros ???; apply E.lt_trans. }
+  Qed.
+
+  Lemma is_sorted_NoDupA {elt} ls
+        (H : @is_sorted elt ls = true)
+  : NoDupA (@eq_key _) ls.
+  Proof.
+    apply Sorted_is_sorted in H.
+    eapply SortA_NoDupA; eauto; typeclasses eauto.
+  Qed.
+
+  Definition sorted_from_internal_elements {elt} (ls : option (list _))
+    := match ls with
+         | Some ls' => if @is_sorted elt ls'
+                       then Some (from_internal_elements ls')
+                       else None
+         | None => None
+       end.
+
   Local Instance Serializable_map {elt} `{Serializable elt} : Serializable (t elt)
     := {| to_string x := to_string (M.elements x) |}.
 
   Local Instance Deserializable_map {elt} `{Deserializable elt} : Deserializable (t elt)
     := {| from_string s := prod_map
-                             (option_map from_internal_elements)
+                             (sorted_from_internal_elements)
                              id
                              (from_string (A := list (M.key * (nat * option elt))) s) |}.
 
@@ -1725,44 +1878,19 @@ Module MakeSerializableMergableMap (E : SerializableOrderedType) (M : Sfun E) <:
   Qed.
 
   Lemma adj_elements_2 {elt} eq_elt `{Equivalence elt eq_elt} ls (m : t elt)
-        (HND : NoDupA (@eq_key _) ls)
         (H' : Sorted (@M.lt_key _) ls)
   : M.Equiv (eq * option_lift_relation eq_elt)%signature (from_internal_elements ls) m
     -> eqlistA (E.eq * (eq * option_lift_relation eq_elt))%signature
                ls
                (M.elements m).
   Proof.
+    pose proof (SortA_NoDupA _ _ _ H') as HND.
     rewrite <- adj_elements_equiv; trivial.
     pose proof (M.elements_3 m).
     eapply SortA_equivlistA_eqlistA;
       try eassumption;
       try typeclasses eauto.
     { split; typeclasses eauto. }
-    { split; unfold M.lt_key; simpl.
-      { intros ? H1; apply E.lt_not_eq in H1.
-        apply (H1 (E.eq_refl _)). }
-      { repeat intro; eapply E.lt_trans; eassumption. } }
-    { repeat intro; destruct_head_hnf and; hnf in *;
-      cleanup;
-      hnf in *; simpl in *;
-      add_facts;
-      match goal with
-        | [ H : E.eq ?a ?b, H' : E.lt ?b ?c, H'' : E.eq ?c ?d |- E.lt ?a ?d ]
-          => destruct (E.compare a d); trivial; destruct (E.compare a c); destruct (E.compare b d)
-      end;
-      repeat match goal with
-               | [ H : False |- _ ] => destruct H
-               | [ H : E.eq ?x ?y |- _ ]
-                 => unique pose proof (E.eq_sym H)
-               | [ x : key |- _ ]
-                 => unique pose proof (E.eq_refl x)
-               | [ H : E.eq ?x ?y, H' : E.eq ?y ?z |- _ ]
-                 => unique pose proof (E.eq_trans H H')
-               | [ H : E.lt ?x ?y, H' : E.lt ?y ?z |- _ ]
-                 => unique pose proof (E.lt_trans H H')
-               | [ H : E.lt ?x ?y, H' : E.eq ?x ?y |- _ ]
-                 => unique pose proof (E.lt_not_eq H H')
-             end. }
   Qed.
 
   Lemma MEquiv_Equiv {elt} (eq_elt : relation elt) m1 m2
@@ -1803,13 +1931,20 @@ Module MakeSerializableMergableMap (E : SerializableOrderedType) (M : Sfun E) <:
     intros; simpl; unfold id.
     set (R := (eqlistA (E.eq * (eq * (option_lift_relation eq_elt)))%signature) : relation (list (M.key * (nat * option elt)))).
     split.
-    { simpl.
+    { unfold sorted_from_internal_elements.
+      simpl.
       pose proof (@from_to_string_1 _ R _ (M.elements x)).
+      pose proof (M.elements_3 x).
       repeat match goal with
                | _ => intro
                | _ => progress cleanup
                | _ => progress unfold option_map in *
                | _ => progress simpl in *
+               | [ H : is_sorted _ = false |- _ ] => apply not_Sorted_is_sorted in H
+               | [ H : R ?x ?y, H' : Sorted _ ?y |- _ ]
+                 => unique pose proof (proj2 (Sorted_eqlistA H) H')
+               | [ H : R ?x ?y, H' : Sorted _ ?x |- _ ]
+                 => unique pose proof (proj1 (Sorted_eqlistA H) H')
                | [ |- appcontext[match ?E with _ => _ end] ]
                  => case_eq E
                | [ H : ?x = @None ?T, H' : appcontext G[?x] |- _ ]
@@ -1826,16 +1961,18 @@ Module MakeSerializableMergableMap (E : SerializableOrderedType) (M : Sfun E) <:
       apply H'. }
   Qed.
 
-  Lemma prefix_closed_map {elt}
+  Lemma prefix_closed_map_strict {elt}
         (eq_elt : relation elt)
         `{Equivalence elt eq_elt, PrefixSerializable elt eq_elt}
+        (R0 := (eq * (option_lift_relation eq_elt))%signature)
   : forall s1 s2 x,
-      option_lift_relation (Equiv eq_elt) (fst (from_string (A := t elt) s1)) (Some x)
-      -> option_lift_relation (Equiv eq_elt) (fst (from_string (A := t elt) (s1 ++ s2))) (Some x)
+      option_lift_relation (M.Equiv R0) (fst (from_string (A := t elt) s1)) (Some x)
+      -> option_lift_relation (M.Equiv R0) (fst (from_string (A := t elt) (s1 ++ s2))) (Some x)
          /\ snd (from_string (A := t elt) (s1 ++ s2)) = (snd (from_string (A := t elt) s1) ++ s2)%string.
   Proof.
     simpl; unfold id.
-    set (R := (eqlistA (E.eq * (eq * (option_lift_relation eq_elt)))%signature) : relation (list (M.key * (nat * option elt)))).
+    set (R := eqlistA (E.eq * R0)%signature).
+    assert (Reflexive R) by (subst R; typeclasses eauto).
     intros s1 s2 x; split; simpl in *;
     [ assert (H' := @prefix_closed_1 _ R _ s1 s2)
     | assert (H' := @prefix_closed_2 _ R _ s1 s2 (M.elements x)) ];
@@ -1864,12 +2001,46 @@ Module MakeSerializableMergableMap (E : SerializableOrderedType) (M : Sfun E) <:
              | _ => eapply H'; clear H'
              | _ => solve [ subst R; eauto ]
              | _ => solve [ subst R; eauto using adj_elements_2, adj_elements_1 ]
+             | [ H : is_sorted _ = false |- _ ] => apply not_Sorted_is_sorted in H
+             | [ H : is_sorted _ = true |- _ ] => apply Sorted_is_sorted in H
+             | [ H : R ?x ?y, H' : Sorted _ ?y |- _ ]
+               => unique pose proof (proj2 (Sorted_eqlistA H) H')
+             | [ H : R ?x ?y, H' : Sorted _ ?x |- _ ]
+               => unique pose proof (proj1 (Sorted_eqlistA H) H')
+             | [ H : forall _, R _ _ -> R _ _ |- _ ]
+               => unique pose proof (H' _ (reflexivity _))
+             | [ H : ?T, H' : ~?T |- _ ] => destruct (H' H)
            end.
-    admit.
-    exfalso; clear; admit.
-    exfalso; clear; admit.
-    Grab Existential Variables.
-    admit.
+  Qed.
+
+  Lemma prefix_closed_map {elt}
+        (eq_elt : relation elt)
+        `{Equivalence elt eq_elt, PrefixSerializable elt eq_elt}
+  : forall s1 s2 x,
+      option_lift_relation (Equiv eq_elt) (fst (from_string (A := t elt) s1)) (Some x)
+      -> option_lift_relation (Equiv eq_elt) (fst (from_string (A := t elt) (s1 ++ s2))) (Some x)
+         /\ snd (from_string (A := t elt) (s1 ++ s2)) = (snd (from_string (A := t elt) s1) ++ s2)%string.
+  Proof.
+    intros s1 s2 x.
+    pose proof (@prefix_closed_map_strict elt eq_elt _ _ s1 s2).
+    repeat match goal with
+             | _ => progress unfold option_lift_relation
+             | _ => progress unfold id in *
+             | [ H : ?x = Some _, H' : appcontext[?x] |- _ ] => rewrite H in H'
+             | [ H : ?x = None, H' : appcontext[?x] |- _ ] => rewrite H in H'
+             | _ => progress simpl in *
+             | [ H : appcontext[match ?E with _ => _ end] |- _ ]
+               => revert H; case_eq E; intros
+             | [ |- appcontext[match ?E with _ => _ end] ]
+               => case_eq E; intros
+             | [ H : forall x, M.Equiv _ _ _ -> _ |- _ ]
+               => specialize (H _ (reflexivity _))
+             | _ => progress split_and
+             | [ H : False |- _ ] => destruct H
+             | [ H : M.Equiv _ _ _ |- _ ] => apply MEquiv_Equiv in H
+             | [ |- _ /\ _ ] => split; eauto; []
+             | _ => solve [ etransitivity; eauto ]
+           end.
   Qed.
 
   Definition PrefixSerializable_map {elt} {eq_elt} `{Equivalence elt eq_elt, PrefixSerializable elt eq_elt}
